computation/compute_atmost_k_steps.v
@@ -1,0 +1,108 @@
+(*
+
+  Copyright 2014 Cornell University
+  Copyright 2015 Cornell University
+  Copyright 2016 Cornell University
+  Copyright 2017 Cornell University
+
+  This file is part of VPrl (the Verified Nuprl project).
+
+  VPrl is free software: you can redistribute it and/or modify
+  it under the terms of the GNU General Public License as published by
+  the Free Software Foundation, either version 3 of the License, or
+  (at your option) any later version.
+
+  VPrl is distributed in the hope that it will be useful,
+  but WITHOUT ANY WARRANTY; without even the implied warranty of
+  MERCHANTABILITY or FITNESS FOR A PARTICULAR PURPOSE.  See the
+  GNU General Public License for more details.
+
+  You should have received a copy of the GNU General Public License
+  along with VPrl.  If not, see <http://www.gnu.org/licenses/>.
+
+
+  Websites: http://nuprl.org/html/verification/
+            http://nuprl.org/html/Nuprl2Coq
+            https://github.com/vrahli/NuprlInCoq
+
+  Authors: Vincent Rahli
+
+*)
+
+
+Require Export computation2.
+
+
+Fixpoint compute_atmost_k_steps {o}
+         (lib : library)
+         (k   : nat)
+         (t   : @NTerm o) : NTerm :=
+  match k with
+    | 0 => t
+    | S n =>
+      match compute_step lib t with
+      | csuccess u => compute_atmost_k_steps lib n u
+      | cfailure _ _ => t
+      end
+  end.
+
+Lemma reduces_atmost_k_steps_of_compute_atmost_k_steps {o} :
+  forall lib k (t : @NTerm o),
+    {n : nat
+     & n <= k
+     # reduces_in_atmost_k_steps lib t (compute_atmost_k_steps lib k t) n}.
+Proof.
+  induction k; introv; simpl.
+
+  - exists 0; dands; auto.
+    rw @reduces_in_atmost_k_steps_0; auto.
+
+  - remember (compute_step lib t) as comp; symmetry in Heqcomp.
+    destruct comp as [u|].
+
+    + pose proof (IHk u) as h; clear IHk; exrepnd.
+      exists (S n); dands; auto; try omega.
+      rw @reduces_in_atmost_k_steps_S; allrw.
+      eexists; dands; eauto.
+
+    + exists 0; dands; try omega.
+      rw @reduces_in_atmost_k_steps_0; auto.
+Qed.
+
+Lemma reduces_to_of_compute_atmost_k_steps {o} :
+  forall lib k (t : @NTerm o),
+    reduces_to lib t (compute_atmost_k_steps lib k t).
+Proof.
+  introv.
+  pose proof (reduces_atmost_k_steps_of_compute_atmost_k_steps lib k t) as q; exrepnd.
+  exists n; auto.
+Qed.
+
+Definition sonobnd {o} (t : @SOTerm o) : SOBTerm := sobterm [] t.
+
+Definition mk_so_equality {o} (t1 t2 T : @SOTerm o) :=
+  soterm (Can NEquality) [sonobnd t1, sonobnd t2, sonobnd T].
+
+Definition opabs_member : opabs := Build_opabs "member" [] [0,0].
+
+(* It would be better if the proof was just eq_refl *)
+Lemma opabs_member_correct {o} :
+  @correct_abs
+    o
+    opabs_member
+    [(nvart, 0), (nvarT, 0)]
+    (mk_so_equality (sovar nvart []) (sovar nvart []) (sovar nvarT [])).
+Proof.
+  exact (eq_refl, (eq_refl, (eq_refl, (eq_refl, eq_refl)))).
+Qed.
+
+Definition mk_abs {o} abs (l : list (@BTerm o)) : NTerm := oterm (Abs abs) l.
+
+Time Eval compute in (compute_atmost_k_steps
+                        [lib_abs
+                           opabs_member
+                           [(nvart, 0), (nvarT, 0)]
+                           (mk_so_equality (sovar nvart []) (sovar nvart []) (sovar nvarT []))
+                           opabs_member_correct]
+                        1
+                        (mk_abs opabs_member [nobnd (mk_var (nvar "t")), nobnd (mk_var (nvar "T"))])).
